\documentclass[main.tex]{subfiles}

\everymath{\displaystyle}
\begin{document}
  
\tiny

\begin{tabular}{cl}
  \toprule
  \\Partial Fraction Decomposition &
  $
  \begin{array}{lr}
    F(s) = \frac{N(s)}{D(s)}
    = \sum_{i=0}^n \sum_{k=1}^r \frac{K_{ik}}{(s+p_i)^k}
    \\\mathrm{K}_{ik} = \lim\limits_{s \to -p_i} \frac{1}{(r-k)!}
    \mathcal{D}^{r-k}[\frac{\mathrm{N}(s)}{\mathrm{D(s)}}(s-p_i)^r]
  \end{array}
  $
  \\\midrule
  \\Transfer Function &
  $ 
  \begin{array}{ll}
    L(c) = L(r)
    \\G(s) 
      = \frac{C(s)}{R(s)} 
      = \frac{\Lap{P_{dr}}}{\Lap{P_{dc}}}
      = \frac{\Lap{c(t)}}{\Lap{r(t)}}
  \end{array}
  $
  \\\midrule
  \\Electrical Analysis &
  \begin{tabular}{lc}
    Time Model & S-Model (Impedance)
    \\$i(t) = Rv(t)$ & $R$ 
    \\$i(t) = CD[v(t)] $ & $\frac{1}{Cs}$ 
    \\$v(t) = LD[i(t)]$ & $Ls$
  \end{tabular}
  \\\midrule
  \\Mechanical Analysis &
  \begin{tabular}{lcl}
    Time Model & S-Model (Impedance) &
    \\$f(t) = Kx(t)$ & $K$ & Spring
    \\$f(t) = \mathrm{f}_vD[x(t)]$ & $\mathrm{f}_vs$ & Damper
    \\$f(t) = MD^2[x(t)]$ & $Ms^2$ & Mass (Newton's 1st law)
  \end{tabular}
  \\\midrule
  \\Mechatronics Analysis &
  $
	  G(s) = \frac{\theta(s)}{v(s)} 
    \approx \left. \frac{K}{s+a} \right| 
      K = \frac{K_t}{Ri(s)}, a = \frac{D_m+\frac{K_tK_b}{R}}{i(s)}
  $
	\\\midrule
	\\Second Order Linear System &
	\begin{tabular}{lc}
		General Form & $\frac{\omega_n^2}{s^2+2\omega_n\xi s+\omega_n^2}$
		\\ $\xi$      & $\left. \frac{\alpha}{2\omega_n} \right| \alpha =2\omega_n\xi$
		\\ $\omega_n$ & $\left. \sqrt{\beta} \right| \beta = \omega_n^2$
		\\ $T_p$      & $\frac{\pi}{\omega_n \sqrt{1-\xi^2}}$
		\\ $T_s$      & $\\frac{4}{\omega_n\xi}$
		\\\%OS       & $100\e^{-\xi\omega_n T_p}$
	\end{tabular}
	\\\midrule
	\\Damping Characteristics &
	\begin{tabular}{lc}
		overdamped & $\xi > 1$
		\\critically damped & $\xi =1$
		\\under damped & $0 < \xi < 1$
		\\zero damping & $\xi = 0$
		\\unstable & $\xi < 0$
	\end{tabular}
  \\\midrule
  \\Notation &
  $
		\begin{array}{ll}
			  L(y) = (P_{dy})y = \left(a_n(t)D^n + a_{n-1}(t)D^{n-1} + \cdots + a_1(t)D + a_0(t) \right)y
			\\ D^{n}y = \frac{\del{^ny}}{\del{t^n}}
		\end{array}
  $

\\\bottomrule
\end{tabular}

\end{document}
